rasimpl: support got GAST

theories/autosubst/GAST_rasimpl.v
@@ -1,12 +1,522 @@
 (** GAST support for rasimpl **)
 
 From Coq Require Import Utf8 List.
-From GhostTT.autosubst Require Import core unscoped GAST CCAST RAsimpl.
+From GhostTT.autosubst Require Import core unscoped GAST RAsimpl.
 From Coq Require Import Setoid Morphisms Relation_Definitions.
 Import ListNotations.
 
-(* GAST *)
+Inductive quoted_subst :=
+| qsubst_atom (σ : nat → term)
+| qsubst_comp (s t : quoted_subst)
+| qsubst_compr (s : quoted_subst) (r : quoted_ren)
+| qsubst_rcomp (r : quoted_ren) (s : quoted_subst)
+| qsubst_cons (t : quoted_term) (s : quoted_subst)
+| qsubst_id
+| qsubst_ren (r : quoted_ren)
+
+with quoted_term :=
+| qatom (t : term)
+| qren (r : quoted_ren) (t : quoted_term)
+| qsubst (s : quoted_subst) (t : quoted_term).
+
+Fixpoint unquote_subst q :=
+  match q with
+  | qsubst_atom σ => σ
+  | qsubst_comp s t => funcomp (subst_term (unquote_subst s)) (unquote_subst t)
+  | qsubst_compr s r => funcomp (unquote_subst s) (unquote_ren r)
+  | qsubst_rcomp r s => funcomp (ren_term (unquote_ren r)) (unquote_subst s)
+  | qsubst_cons t s => scons (unquote_term t) (unquote_subst s)
+  | qsubst_id => var
+  | qsubst_ren r => funcomp var (unquote_ren r)
+  end
+
+with unquote_term q :=
+  match q with
+  | qatom t => t
+  | qren r t => ren_term (unquote_ren r) (unquote_term t)
+  | qsubst s t => subst_term (unquote_subst s) (unquote_term t)
+  end.
+
+(** Evaluation **)
+
+Inductive eval_subst_comp_view : quoted_subst → quoted_subst → Type :=
+| es_id_l s : eval_subst_comp_view qsubst_id s
+| es_id_r s : eval_subst_comp_view s qsubst_id
+| es_comp_r s u v : eval_subst_comp_view s (qsubst_comp u v)
+| es_compr_r s x y : eval_subst_comp_view s (qsubst_compr x y)
+| es_rcomp_r s x y : eval_subst_comp_view s (qsubst_rcomp x y)
+| es_cons_r s t s' : eval_subst_comp_view s (qsubst_cons t s')
+| es_ren_l r s : eval_subst_comp_view (qsubst_ren r) s
+| es_ren_r s r : eval_subst_comp_view s (qsubst_ren r)
+| es_other u v : eval_subst_comp_view u v.
+
+Definition eval_subst_comp_c u v : eval_subst_comp_view u v :=
+  match u, v with
+  | qsubst_id, v => es_id_l v
+  | u, qsubst_id => es_id_r u
+  | u, qsubst_comp x y => es_comp_r u x y
+  | u, qsubst_compr x y => es_compr_r u x y
+  | u, qsubst_rcomp x y => es_rcomp_r u x y
+  | u, qsubst_cons t s => es_cons_r u t s
+  | qsubst_ren r, s => es_ren_l r s
+  | u, qsubst_ren r => es_ren_r u r
+  | u, v => es_other u v
+  end.
+
+Inductive eval_subst_compr_view : quoted_subst → quoted_ren → Type :=
+| esr_id_l r : eval_subst_compr_view qsubst_id r
+| esr_id_r s : eval_subst_compr_view s qren_id
+| esr_comp_r s x y : eval_subst_compr_view s (qren_comp x y)
+| esr_cons_r s n r : eval_subst_compr_view s (qren_cons n r)
+| esr_ren_l s r : eval_subst_compr_view (qsubst_ren s) r
+| esr_cons_shift t s : eval_subst_compr_view (qsubst_cons t s) qren_shift
+| esr_other s r : eval_subst_compr_view s r.
+
+Definition eval_subst_compr_c s r : eval_subst_compr_view s r :=
+  match s, r with
+  | qsubst_id, r => esr_id_l r
+  | s, qren_id => esr_id_r s
+  | s, qren_comp x y => esr_comp_r s x y
+  | s, qren_cons n r => esr_cons_r s n r
+  | qsubst_ren s, r => esr_ren_l s r
+  | qsubst_cons t s, qren_shift => esr_cons_shift t s
+  | s, r => esr_other s r
+  end.
+
+Inductive eval_subst_rcomp_view : quoted_ren → quoted_subst → Type :=
+| ers_id_l s : eval_subst_rcomp_view qren_id s
+| ers_id_r r : eval_subst_rcomp_view r qsubst_id
+| ers_comp_r r x y : eval_subst_rcomp_view r (qsubst_comp x y)
+| ers_compr_r r x y : eval_subst_rcomp_view r (qsubst_compr x y)
+| ers_rcomp_r r x y : eval_subst_rcomp_view r (qsubst_rcomp x y)
+| ers_cons_r r t s : eval_subst_rcomp_view r (qsubst_cons t s)
+| ers_ren_r r s : eval_subst_rcomp_view r (qsubst_ren s)
+| ers_other r s : eval_subst_rcomp_view r s.
+
+Definition eval_subst_rcomp_c r s : eval_subst_rcomp_view r s :=
+  match r, s with
+  | qren_id, s => ers_id_l s
+  | r, qsubst_id => ers_id_r r
+  | r, qsubst_comp x y => ers_comp_r r x y
+  | r, qsubst_compr x y => ers_compr_r r x y
+  | r, qsubst_rcomp x y => ers_rcomp_r r x y
+  | r, qsubst_cons t s => ers_cons_r r t s
+  | r, qsubst_ren s => ers_ren_r r s
+  | r, s => ers_other r s
+  end.
+
+Inductive qsubst_ren_id_view : quoted_subst → Type :=
+| is_qsubst_ren r : qsubst_ren_id_view (qsubst_ren r)
+| is_qsubst_id : qsubst_ren_id_view qsubst_id
+| not_qsubst_ren_id s : qsubst_ren_id_view s.
+
+Definition test_qsubst_ren_id s : qsubst_ren_id_view s :=
+  match s with
+  | qsubst_ren r => is_qsubst_ren r
+  | qsubst_id => is_qsubst_id
+  | s => not_qsubst_ren_id s
+  end.
+
+(* TODO Could be improved like apply_ren *)
+Fixpoint apply_subst (s : quoted_subst) (n : quoted_nat) : quoted_term :=
+  match s, n with
+  | qsubst_atom s, _ => qatom (s (unquote_nat n))
+  | qsubst_id, _ => qatom (var (unquote_nat n))
+  | _, qnat_atom n => qatom (unquote_subst s n)
+  | qsubst_comp s1 s2, _ => qsubst s1 (apply_subst s2 n)
+  | qsubst_compr s r, _ => apply_subst s (apply_ren r n)
+  | qsubst_rcomp r s, _ => qren r (apply_subst s n)
+  | qsubst_cons t s, q0 => t
+  | qsubst_cons t s, qS n => apply_subst s n
+  | qsubst_ren r, n => qatom (var (unquote_nat (apply_ren r n)))
+  end.
+
+Fixpoint eval_subst (s : quoted_subst) : quoted_subst :=
+  match s with
+  | qsubst_comp u v =>
+    let u := eval_subst u in
+    let v := eval_subst v in
+    match eval_subst_comp_c u v with
+    | es_id_l v => v
+    | es_id_r u => u
+    | es_comp_r u x y => qsubst_comp (qsubst_comp u x) y
+    | es_compr_r u x y => qsubst_compr (qsubst_comp u x) y
+    | es_rcomp_r u x y => qsubst_comp (qsubst_compr u x) y
+    | es_cons_r u t s => qsubst_cons (qsubst u t) (qsubst_comp u s)
+    | es_ren_l r s => qsubst_rcomp r s
+    | es_ren_r u r => qsubst_compr u r
+    | es_other u v => qsubst_comp u v
+    end
+  | qsubst_compr s r =>
+    let s := eval_subst s in
+    let r := eval_ren r in
+    match eval_subst_compr_c s r with
+    | esr_id_l r => qsubst_ren r
+    | esr_id_r s => s
+    | esr_comp_r s x y => qsubst_compr (qsubst_compr s x) y
+    | esr_cons_r s n r => qsubst_cons (apply_subst s n) (qsubst_compr s r)
+    | esr_ren_l s r => qsubst_ren (qren_comp s r)
+    | esr_cons_shift t s => s
+    | esr_other s r => qsubst_compr s r
+    end
+  | qsubst_rcomp r s =>
+    let r := eval_ren r in
+    let s := eval_subst s in
+    match eval_subst_rcomp_c r s with
+    | ers_id_l s => s
+    | ers_id_r r => qsubst_ren r
+    | ers_comp_r r x y => qsubst_comp (qsubst_rcomp r x) y
+    | ers_compr_r r x y => qsubst_compr (qsubst_rcomp r x) y
+    | ers_rcomp_r r x y => qsubst_rcomp (qren_comp r x) y
+    | ers_cons_r r t s => qsubst_cons (qren r t) (qsubst_rcomp r s)
+    | ers_ren_r r s => qsubst_ren (qren_comp r s)
+    | ers_other r s => qsubst_rcomp r s
+    end
+  | qsubst_cons t s =>
+    let t := eval_term t in
+    let s := eval_subst s in
+    qsubst_cons t s
+  | qsubst_ren r =>
+    let r := eval_ren r in
+    match test_qren_id r with
+    | is_qren_id => qsubst_id
+    | not_qren_id r => qsubst_ren r
+    end
+  | _ => s
+  end
+
+with eval_term (t : quoted_term) : quoted_term :=
+  match t with
+  | qren r t =>
+    let r := eval_ren r in
+    let t := eval_term t in
+    match t with
+    | qsubst s t => qsubst (qsubst_comp (qsubst_ren r) s) t
+    | qren r' t => qren (qren_comp r r') t
+    | _ =>
+      match test_qren_id r with
+      | is_qren_id => t
+      | not_qren_id r => qren r t
+      end
+    end
+  | qsubst s t =>
+    let s := eval_subst s in
+    let t := eval_term t in
+    match t with
+    | qsubst s' t => qsubst (qsubst_comp s s') t
+    | qren r t => qsubst (qsubst_compr s r) t
+    | _ =>
+      match test_qsubst_ren_id s with
+      | is_qsubst_ren r => qren r t
+      | is_qsubst_id => t
+      | not_qsubst_ren_id s => qsubst s t
+      end
+    end
+  | _ => t
+  end.
+
+(** Correctness **)
+
+Lemma apply_subst_sound :
+  ∀ s n,
+    unquote_term (apply_subst s n) = unquote_subst s (unquote_nat n).
+Proof.
+  intros s n.
+  induction s in n |- *.
+  all: try reflexivity.
+  - cbn. destruct n.
+    + reflexivity.
+    + cbn. rewrite IHs2. reflexivity.
+    + cbn. rewrite IHs2. reflexivity.
+  - cbn. destruct n.
+    + reflexivity.
+    + rewrite IHs. rewrite apply_ren_sound. reflexivity.
+    + cbn. rewrite IHs. rewrite apply_ren_sound. reflexivity.
+  - cbn. destruct n.
+    + reflexivity.
+    + cbn. rewrite IHs. reflexivity.
+    + cbn. rewrite IHs. reflexivity.
+  - cbn. destruct n.
+    + reflexivity.
+    + reflexivity.
+    + cbn. rewrite IHs. reflexivity.
+  - cbn. destruct n.
+    + reflexivity.
+    + cbn. rewrite apply_ren_sound. reflexivity.
+    + cbn. rewrite apply_ren_sound. reflexivity.
+Qed.
+
+Ltac set_eval_subst na :=
+  lazymatch goal with
+  | eval_subst_sound : ∀ s : quoted_subst, _ |- context [ eval_subst ?s ] =>
+    let IH := fresh "IH" in
+    pose proof (eval_subst_sound s) as IH ;
+    set (na := eval_subst s) in * ;
+    clearbody na
+  end.
+
+Fixpoint eval_subst_sound s :
+    pointwise_relation _ eq (unquote_subst s) (unquote_subst (eval_subst s))
+
+with eval_term_sound t :
+    unquote_term t = unquote_term (eval_term t).
+Proof.
+  {
+    intros n.
+    destruct s.
+    all: try reflexivity.
+    - cbn. set_eval_subst es1. set_eval_subst es2.
+      destruct eval_subst_comp_c.
+      + cbn in *. unfold funcomp. rewrite IH, IH0.
+        asimpl. reflexivity.
+      + cbn in *. unfold funcomp. rewrite IH, IH0.
+        asimpl. reflexivity.
+      + cbn in *. unfold funcomp in *.
+        erewrite subst_term_morphism. 2,3: eauto.
+        asimpl. reflexivity.
+      + cbn in *. unfold funcomp in *.
+        erewrite subst_term_morphism. 2,3: eauto.
+        asimpl. reflexivity.
+      + cbn in *. unfold funcomp in *.
+        erewrite subst_term_morphism. 2,3: eauto.
+        asimpl. reflexivity.
+      + cbn in *. unfold funcomp.
+        erewrite subst_term_morphism. 2,3: eauto.
+        asimpl. destruct n. all: reflexivity.
+      + cbn in *. unfold funcomp in *.
+        rewrite IH, IH0.
+        rewrite rinstInst'_term. reflexivity.
+      + cbn in *. unfold funcomp in *.
+        rewrite IH, IH0. reflexivity.
+      + cbn in *. unfold funcomp. rewrite IH, IH0. reflexivity.
+    - cbn. set_eval_subst es.
+      remember (eval_ren _) as er eqn:e.
+      destruct eval_subst_compr_c.
+      + subst. cbn. unfold funcomp. rewrite IH.
+        cbn. rewrite <- eval_ren_sound. reflexivity.
+      + unfold funcomp. rewrite eval_ren_sound, <- e. cbn.
+        rewrite IH. reflexivity.
+      + unfold funcomp. rewrite eval_ren_sound, <- e. cbn.
+        rewrite IH. reflexivity.
+      + unfold funcomp. rewrite eval_ren_sound, <- e. cbn.
+        rewrite IH. destruct n. 2: reflexivity.
+        cbn. rewrite apply_subst_sound. reflexivity.
+      + subst. cbn. unfold funcomp. rewrite <- eval_ren_sound.
+        rewrite IH. reflexivity.
+      + unfold funcomp. rewrite eval_ren_sound, <- e. cbn.
+        rewrite IH. cbn. reflexivity.
+      + subst. cbn. unfold funcomp. rewrite <- eval_ren_sound.
+        rewrite IH. reflexivity.
+    - cbn. set_eval_subst es.
+      remember (eval_ren _) as er eqn:e.
+      destruct eval_subst_rcomp_c.
+      + unfold funcomp.
+        erewrite ren_term_morphism. 3: reflexivity.
+        2:{ intro. rewrite eval_ren_sound, <- e. reflexivity. }
+        cbn. asimpl. auto.
+      + subst. unfold funcomp. rewrite IH. cbn. rewrite eval_ren_sound.
+        reflexivity.
+      + subst. unfold funcomp. rewrite IH. cbn. unfold funcomp.
+        rewrite substRen_term. apply subst_term_morphism. 2: reflexivity.
+        intro. unfold funcomp. apply ren_term_morphism. 2: reflexivity.
+        intro. rewrite <- eval_ren_sound. reflexivity.
+      + subst. unfold funcomp. rewrite IH. cbn. unfold funcomp.
+        apply ren_term_morphism. 2: reflexivity.
+        intro. rewrite <- eval_ren_sound. reflexivity.
+      + subst. unfold funcomp. rewrite IH. cbn. unfold funcomp.
+        rewrite renRen_term. apply ren_term_morphism. 2: reflexivity.
+        intro. rewrite <- eval_ren_sound. reflexivity.
+      + subst. unfold funcomp. rewrite IH. cbn.
+        destruct n.
+        * cbn. apply ren_term_morphism. 2: reflexivity.
+          intro. rewrite eval_ren_sound. reflexivity.
+        * cbn. unfold funcomp. apply ren_term_morphism. 2: reflexivity.
+          intro. rewrite eval_ren_sound. reflexivity.
+      + subst. unfold funcomp. rewrite IH. cbn. unfold funcomp.
+        rewrite <- eval_ren_sound. reflexivity.
+      + subst. cbn. unfold funcomp. rewrite IH.
+        apply ren_term_morphism. 2: reflexivity.
+        intro. rewrite eval_ren_sound. reflexivity.
+    - cbn. erewrite scons_morphism. 2,3: eauto.
+      reflexivity.
+    - cbn. remember (eval_ren _) as er eqn:e.
+      destruct test_qren_id.
+      + cbn. unfold funcomp. rewrite eval_ren_sound, <- e.
+        reflexivity.
+      + subst. cbn. unfold funcomp. rewrite <- eval_ren_sound.
+        reflexivity.
+  }
+  {
+    destruct t.
+    - reflexivity.
+    - cbn. remember (eval_term _) as et eqn:e in *.
+      destruct et.
+      + remember (eval_ren _) as rr eqn:er.
+        destruct test_qren_id.
+        * rewrite eval_term_sound, <- e.
+          cbn. erewrite ren_term_morphism. 3: reflexivity.
+          2:{ intro. rewrite eval_ren_sound, <- er. reflexivity. }
+          cbn. asimpl. reflexivity.
+        * subst. cbn. rewrite eval_term_sound, <- e. cbn.
+          eapply ren_term_morphism. 2: reflexivity.
+          intro. apply eval_ren_sound.
+      + cbn. rewrite eval_term_sound, <- e. cbn. rewrite renRen_term.
+        apply ren_term_morphism. 2: reflexivity.
+        intro. unfold funcomp. rewrite <- eval_ren_sound. reflexivity.
+      + cbn. rewrite eval_term_sound, <- e. cbn.
+        rewrite substRen_term.
+        apply subst_term_morphism. 2: reflexivity.
+        intro. unfold funcomp.
+        rewrite rinstInst'_term.
+        apply subst_term_morphism. 2: reflexivity.
+        intro. unfold funcomp.
+        rewrite <- eval_ren_sound. reflexivity.
+    - cbn. remember (eval_term _) as et eqn:e in *.
+      destruct et.
+      + remember (eval_subst _) as ss eqn:es in *.
+        rewrite eval_term_sound, <- e. cbn.
+        destruct test_qsubst_ren_id.
+        * cbn. erewrite subst_term_morphism. 3: reflexivity.
+          2:{ intro. rewrite eval_subst_sound, <- es. reflexivity. }
+          cbn. rewrite rinstInst'_term. reflexivity.
+        * cbn. erewrite subst_term_morphism. 3: reflexivity.
+          2:{ intro. rewrite eval_subst_sound, <- es. reflexivity. }
+          cbn. asimpl. reflexivity.
+        * subst. cbn.
+          eapply subst_term_morphism. 2: reflexivity.
+          intro. apply eval_subst_sound.
+      + cbn. rewrite eval_term_sound, <- e. cbn. rewrite renSubst_term.
+        apply subst_term_morphism. 2: reflexivity.
+        intro. unfold funcomp. rewrite <- eval_subst_sound. reflexivity.
+      + cbn. rewrite eval_term_sound, <- e. cbn. rewrite substSubst_term.
+        eapply subst_term_morphism. 2: reflexivity.
+        intro. unfold funcomp.
+        eapply subst_term_morphism. 2: reflexivity.
+        intro. rewrite <- eval_subst_sound. reflexivity.
+  }
+Qed.
+
+(** Quoting **)
+
+Ltac quote_subst s :=
+  lazymatch s with
+  | funcomp var ?r =>
+    let q := quote_ren r in
+    constr:(qsubst_ren q)
+  | λ x, var (?r x) =>
+    let q := quote_ren r in
+    constr:(qsubst_ren q)
+  | funcomp (subst_term ?s) ?t =>
+    let q := quote_subst s in
+    let q' := quote_subst t in
+    constr:(qsubst_comp q q')
+  | λ x, subst_term ?s (?t x) =>
+    let q := quote_subst s in
+    let q' := quote_subst t in
+    constr:(qsubst_comp q q')
+  | funcomp (ren_term ?r) ?s =>
+    let qr := quote_ren r in
+    let qs := quote_subst s in
+    constr:(qsubst_rcomp qr qs)
+  | funcomp ?s ?r =>
+    let qs := quote_subst s in
+    let qr := quote_ren r in
+    constr:(qsubst_compr qs qr)
+  | λ x, ?s (?r x) =>
+    let qs := quote_subst s in
+    let qr := quote_ren r in
+    constr:(qsubst_compr qs qr)
+  | scons ?t ?s =>
+    let qt := quote_term t in
+    let q := quote_subst s in
+    constr:(qsubst_cons qt q)
+  | ids => constr:(qsubst_id)
+  | var => constr:(qsubst_id)
+  | _ => constr:(qsubst_atom s)
+  end
+
+with quote_term t :=
+  lazymatch t with
+  | ren_term ?r ?t =>
+    let qr := quote_ren r in
+    let qt := quote_term t in
+    constr:(qren qr qt)
+  | subst_term ?s ?t =>
+    let qs := quote_subst s in
+    let qt := quote_term t in
+    constr:(qsubst qs qt)
+  | _ => constr:(qatom t)
+  end.
+
+(** Unfoldings **)
+
 #[export] Hint Unfold
   VarInstance_term Ren_term Up_term_term Up_term up_term Subst_term
   upRen_term_term up_term_term
   : asimpl_unfold.
+
+Class TermSimplification (t s : term) := MkSimplTm {
+  autosubst_simpl_term : t = s
+}.
+
+Arguments autosubst_simpl_term t {s _}.
+
+Hint Mode TermSimplification + - : typeclass_instances.
+
+Declare Reduction asimpl_cbn_term :=
+  cbn [
+    unquote_term eval_term test_qren_id test_qsubst_ren_id
+    unquote_ren eval_ren apply_ren eval_ren_comp_c
+    unquote_subst eval_subst eval_subst_compr_c eval_subst_comp_c
+    eval_subst_rcomp_c apply_subst
+    unquote_nat
+    ren_term subst_term scons
+  ].
+
+Declare Reduction asimpl_unfold_term :=
+  unfold upRen_term_term, up_ren, up_term_term, var_zero.
+
+#[export] Hint Extern 10 (TermSimplification ?t _) =>
+  let q := quote_term t in
+  let s := eval asimpl_cbn_term in (unquote_term (eval_term q)) in
+  let s := eval asimpl_unfold_term in s in
+  exact (MkSimplTm t s (eval_term_sound q))
+  : typeclass_instances.
+
+Class SubstSimplification (r s : nat → term) := MkSimplSubst {
+  autosubst_simpl_csubst : pointwise_relation _ eq r s
+}.
+
+Arguments autosubst_simpl_csubst r {s _}.
+
+Hint Mode SubstSimplification + - : typeclass_instances.
+
+#[export] Hint Extern 10 (SubstSimplification ?r _) =>
+  let q := quote_subst r in
+  let s := eval asimpl_cbn_term in (unquote_subst (eval_subst q)) in
+  let s := eval asimpl_unfold_term in s in
+  exact (MkSimplSubst r s (eval_subst_sound q))
+  : typeclass_instances.
+
+Lemma autosubst_simpl_term_ren :
+  ∀ r t s,
+    TermSimplification (ren_term r t) s →
+    ren_term r t = s.
+Proof.
+  intros r t s H.
+  apply autosubst_simpl_term, _.
+Qed.
+
+Lemma autosubst_simpl_term_subst :
+  ∀ r t s,
+    TermSimplification (subst_term r t) s →
+    subst_term r t = s.
+Proof.
+  intros r t s H.
+  apply autosubst_simpl_term, _.
+Qed.
+
+(** Triggers **)
+
+#[export] Hint Rewrite -> autosubst_simpl_term_ren : asimpl.
+#[export] Hint Rewrite -> autosubst_simpl_term_subst : asimpl.
